theories/std/channel1.v
@@ -1,0 +1,288 @@
+From heap_lang Require Import
+  prelude.
+From heap_lang.iris.base_logic Require Import
+  lib.oneshot
+  lib.excl.
+From heap_lang.language Require Import
+  notations
+  proofmode.
+From heap_lang.std Require Import
+  record3.
+From heap_lang.std Require Export
+  condition.
+
+Implicit Types b : bool.
+Implicit Types l : loc.
+
+#[local] Notation "t '.[flag]'" :=
+  t.[0]%stdpp
+( at level 5
+) : stdpp_scope.
+#[local] Notation "t '.[mutex]'" :=
+  t.[1]%stdpp
+( at level 5
+) : stdpp_scope.
+#[local] Notation "t '.[condition]'" :=
+  t.[2]%stdpp
+( at level 5
+) : stdpp_scope.
+#[local] Notation "t '.[flag]'" :=
+  t.[#0]%E
+( at level 5
+) : expr_scope.
+#[local] Notation "t '.[mutex]'" :=
+  t.[#1]%E
+( at level 5
+) : expr_scope.
+#[local] Notation "t '.[condition]'" :=
+  t.[#2]%E
+( at level 5
+) : expr_scope.
+
+Section condition.
+  Context `{heap_GS : !heapGS Σ} {mutex : mutex Σ} (condition : condition mutex).
+
+  Definition channel1_create : val :=
+    λ: <>,
+      let: "t" := record3_make #false #() #() in
+      "t".[mutex] <- mutex.(mutex_create) #() ;;
+      "t".[condition] <- condition.(condition_create) #() ;;
+      "t".
+
+  Definition channel1_signal : val :=
+    λ: "t",
+      mutex.(mutex_protect) !"t".[mutex] (λ: <>,
+        "t".[flag] <- #true
+      ) ;;
+      condition.(condition_signal) !"t".[condition].
+
+  Definition channel1_wait : val :=
+    λ: "t",
+      let: "mtx" := !"t".[mutex] in
+      let: "cond" := !"t".[condition] in
+      mutex.(mutex_protect) "mtx" (λ: <>,
+        condition.(condition_wait_until) "cond" "mtx" (λ: <>, !"t".[flag])
+      ).
+End condition.
+
+Class Channel1G Σ `{heap_GS : !heapGS Σ} := {
+  #[local] channel1_G_producer_G :: OneshotG Σ unit unit ;
+  #[local] channel1_G_consumer_G :: ExclG Σ unitO ;
+}.
+
+Definition channel1_Σ := #[
+  oneshot_Σ unit unit ;
+  excl_Σ unitO
+].
+#[global] Instance subG_channel1_Σ Σ `{heap_GS : !heapGS Σ} :
+  subG channel1_Σ Σ →
+  Channel1G Σ .
+Proof.
+  solve_inG.
+Qed.
+
+Section channel1_G.
+  Context `{channel1_G : Channel1G Σ}.
+  Context {mutex : mutex Σ} (condition : condition mutex).
+
+  Record channel1_meta := {
+    channel1_meta_producer : gname ;
+    channel1_meta_consumer : gname ;
+  }.
+  Implicit Types γ : channel1_meta.
+
+  #[local] Instance channel1_meta_eq_dec : EqDecision channel1_meta :=
+    ltac:(solve_decision).
+  #[local] Instance channel1_meta_countable :
+    Countable channel1_meta.
+  Proof.
+    pose encode γ := (
+      γ.(channel1_meta_producer),
+      γ.(channel1_meta_consumer)
+    ).
+    pose decode := λ '(γ_producer, γ_consumer), {|
+      channel1_meta_producer := γ_producer ;
+      channel1_meta_consumer := γ_consumer ;
+    |}.
+    refine (inj_countable' encode decode _). intros []. done.
+  Qed.
+
+  #[local] Definition channel1_inv_inner l γ P : iProp Σ :=
+    ∃ b,
+    l.[flag] ↦ #b ∗
+    if b then
+      oneshot_shot γ.(channel1_meta_producer) () ∗
+      ( P
+      ∨ excl γ.(channel1_meta_consumer) ()
+      )
+    else
+      oneshot_pending γ.(channel1_meta_producer) (DfracOwn (1/3)) ().
+  #[local] Definition channel1_inv t P : iProp Σ :=
+    ∃ l γ mtx cond,
+    ⌜t = #l⌝ ∗
+    meta l nroot γ ∗
+    l.[mutex] ↦□ mtx ∗
+    mutex.(mutex_inv) mtx (channel1_inv_inner l γ P) ∗
+    l.[condition] ↦□ cond ∗
+    condition.(condition_inv) cond.
+
+  Definition channel1_producer t : iProp Σ :=
+    ∃ l γ,
+    ⌜t = #l⌝ ∗
+    meta l nroot γ ∗
+    oneshot_pending γ.(channel1_meta_producer) (DfracOwn (2/3)) ().
+
+  Definition channel1_consumer t : iProp Σ :=
+    ∃ l γ,
+    ⌜t = #l⌝ ∗
+    meta l nroot γ ∗
+    excl γ.(channel1_meta_consumer) ().
+
+  #[global] Instance channel1_inv_persistent t P :
+    Persistent (channel1_inv t P).
+  Proof.
+    apply _.
+  Qed.
+  #[global] Instance channel1_producer_timeless t :
+    Timeless (channel1_producer t).
+  Proof.
+    apply _.
+  Qed.
+  #[global] Instance channel1_consumer_timeless t :
+    Timeless (channel1_consumer t).
+  Proof.
+    apply _.
+  Qed.
+
+  Lemma channel1_producer_exclusive t :
+    channel1_producer t -∗
+    channel1_producer t -∗
+    False.
+  Proof.
+    iIntros "(%l & %γ & -> & #Hmeta & Hpending) (%_l & %_γ & %Heq & _Hmeta & Hpending')". injection Heq as <-.
+    iDestruct (meta_agree with "Hmeta _Hmeta") as %<-. iClear "_Hmeta".
+    iDestruct (oneshot_pending_valid_2 with "Hpending Hpending'") as %(? & _). done.
+  Qed.
+
+  Lemma channel1_consumer_exclusive t :
+    channel1_consumer t -∗
+    channel1_consumer t -∗
+    False.
+  Proof.
+    iIntros "(%l & %γ & -> & #Hmeta & Hexcl) (%_l & %_γ & %Heq & _Hmeta & Hexcl')". injection Heq as <-.
+    iDestruct (meta_agree with "Hmeta _Hmeta") as %<-. iClear "_Hmeta".
+    iDestruct (excl_exclusive with "Hexcl Hexcl'") as %[].
+  Qed.
+
+  Lemma channel1_create_spec P :
+    {{{ True }}}
+      channel1_create condition #()
+    {{{ t,
+      RET t;
+      channel1_inv t P ∗
+      channel1_producer t ∗
+      channel1_consumer t
+    }}}.
+  Proof.
+    iIntros "%Φ _ HΦ".
+
+    wp_rec.
+
+    wp_apply (record3_make_spec with "[//]"). iIntros "%l (Hl & Hmeta)".
+    iDestruct (record3_model_eq_1 with "Hl") as "(Hflag & Hmtx & Hcond)".
+
+    iMod (oneshot_alloc ()) as "(%γ_producer & Hpending)".
+    iEval (assert (1 = 2/3 + 1/3)%Qp as -> by compute_done) in "Hpending".
+    iDestruct "Hpending" as "(Hpending1 & Hpending2)".
+
+    iMod (excl_alloc (excl_G := channel1_G_consumer_G) ()) as "(%γ_consumer & Hexcl)".
+
+    pose γ := {|
+      channel1_meta_producer := γ_producer ;
+      channel1_meta_consumer := γ_consumer ;
+    |}.
+    iMod (meta_set _ _ γ nroot with "Hmeta") as "#Hmeta"; first done.
+
+    wp_smart_apply (mutex_create_spec _ (channel1_inv_inner l γ P) with "[Hflag Hpending2]"); first iSteps. iIntros "%mtx #Hmtx_inv".
+    wp_store.
+    iMod (mapsto_persist with "Hmtx") as "Hmtx".
+
+    wp_smart_apply (condition_create_spec _ with "[//]"). iIntros "%cond #Hcond_inv".
+    wp_store.
+    iMod (mapsto_persist with "Hcond") as "Hcond".
+
+    iSteps.
+  Qed.
+
+  Lemma channel1_signal_spec t P :
+    {{{
+      channel1_inv t P ∗
+      channel1_producer t ∗
+      P
+    }}}
+      channel1_signal condition t
+    {{{
+      RET #(); True
+    }}}.
+  Proof.
+    iIntros "%Φ ((%l & %γ & %mtx & %cond & -> & #Hmeta & #Hmtx & #Hmtx_inv & #Hcond & #Hcond_inv) & (%_l & %_γ & %Heq & _Hmeta & Hpending) & HP) HΦ". injection Heq as <-.
+    iDestruct (meta_agree with "Hmeta _Hmeta") as %<-. iClear "_Hmeta".
+    wp_rec.
+    wp_load.
+    wp_apply (mutex_protect_spec _ (λ _, True%I) with "[$Hmtx_inv Hpending HP]").
+    { iIntros "Hmtx_locked (%b & Hflag & Hb)". destruct b.
+      - iDestruct "Hb" as "(Hshot & _)".
+        iDestruct (oneshot_pending_shot with "Hpending Hshot") as %[].
+      - iCombine "Hpending Hb" as "Hpending".
+        assert (2/3 + 1/3 = 1)%Qp as -> by compute_done.
+        iMod (oneshot_update_shot with "Hpending") as "Hshot".
+        iSteps.
+    }
+    iIntros "% _".
+    wp_load.
+    wp_apply (condition_signal_spec with "Hcond_inv").
+    iSteps.
+  Qed.
+
+  Lemma channel1_wait_spec t P :
+    {{{
+      channel1_inv t P ∗
+      channel1_consumer t
+    }}}
+      channel1_wait condition t
+    {{{
+      RET #();
+      P
+    }}}.
+  Proof.
+    iIntros "%Φ ((%l & %γ & %mtx & %cond & -> & #Hmeta & #Hmtx & #Hmtx_inv & #Hcond & #Hcond_inv) & (%_l & %_γ & %Heq & _Hmeta & Hexcl)) HΦ". injection Heq as <-.
+    iDestruct (meta_agree with "Hmeta _Hmeta") as %<-. iClear "_Hmeta".
+    wp_rec.
+    do 2 wp_load.
+    wp_smart_apply (mutex_protect_spec _ (λ res, ⌜res = #()⌝ ∗ P)%I with "[$Hmtx_inv Hexcl]").
+    { iIntros "Hmtx_locked Hsignal_inv".
+      pose (Ψ b := (
+        if b then
+          P
+        else
+          excl γ.(channel1_meta_consumer) ()
+      )%I).
+      wp_smart_apply (condition_wait_until_spec _ Ψ with "[$Hcond_inv $Hmtx_inv $Hmtx_locked $Hsignal_inv $Hexcl]").
+      { clear. iStep 15 as (Φ b) "Hb Hexcl Hflag".
+        destruct b; last iSteps.
+        iDestruct "Hb" as "(Hshot & [Hmodel | Hexcl'])"; first iSmash.
+        iDestruct (excl_exclusive with "Hexcl Hexcl'") as %[].
+      }
+      iSteps.
+    }
+    iSteps.
+  Qed.
+End channel1_G.
+
+#[global] Opaque channel1_create.
+#[global] Opaque channel1_wait.
+#[global] Opaque channel1_signal.
+
+#[global] Opaque channel1_inv.
+#[global] Opaque channel1_producer.
+#[global] Opaque channel1_consumer.
