theories/std/condition.v
@@ -1,0 +1,167 @@
+From heap_lang Require Import
+  prelude.
+From heap_lang.language Require Import
+  notations
+  proofmode.
+From heap_lang.std Require Export
+  mutex.
+
+Implicit Types cond : val.
+
+Record condition `{heap_GS : !heapGS Σ} {mutex : mutex Σ} := {
+  condition_create : val ;
+  condition_wait : val ;
+  condition_signal : val ;
+  condition_broadcast : val ;
+
+  condition_inv : val → iProp Σ ;
+
+  #[global] condition_inv_persistent t ::
+    Persistent (condition_inv t) ;
+
+  condition_create_spec :
+    {{{ True }}}
+      condition_create #()
+    {{{ t,
+      RET t;
+      condition_inv t
+    }}} ;
+
+  condition_wait_spec t mtx P :
+    {{{
+      condition_inv t ∗
+      mutex.(mutex_inv) mtx P ∗
+      mutex.(mutex_locked) mtx ∗
+      P
+    }}}
+      condition_wait t mtx
+    {{{
+      RET #();
+      mutex.(mutex_locked) mtx ∗
+      P
+    }}} ;
+
+  condition_signal_spec t :
+    {{{
+      condition_inv t
+    }}}
+      condition_signal t
+    {{{
+      RET #(); True
+    }}} ;
+
+  condition_broadcast_spec t :
+    {{{
+      condition_inv t
+    }}}
+      condition_broadcast t
+    {{{
+      RET #(); True
+    }}} ;
+}.
+#[global] Arguments condition {_ _} _ : assert.
+#[global] Arguments Build_condition {_ _ _ _ _ _ _ _ _} _ _ _ _ : assert.
+
+Section condition.
+  Context `{heap_GS : !heapGS Σ} {mutex : mutex Σ} (condition : condition mutex).
+
+  #[local] Definition condition_wait_until_aux : val :=
+    rec: "condition_wait_until_aux" "t" "mtx" "cond" :=
+      if: "cond" #() then #() else (
+        condition.(condition_wait) "t" "mtx" ;;
+        "condition_wait_until_aux" "t" "mtx" "cond"
+      ).
+  Definition condition_wait_until : val :=
+    λ: "t" "mtx" "cond",
+      condition_wait_until_aux "t" "mtx" "cond".
+
+  Definition condition_wait_while : val :=
+    λ: "t" "mtx" "cond",
+      condition_wait_until "t" "mtx" (λ: <>, ~ "cond" #()).
+
+  Lemma condition_wait_until_spec Ψ t mtx cond P :
+    {{{
+      condition.(condition_inv) t ∗
+      mutex.(mutex_inv) mtx P ∗
+      mutex.(mutex_locked) mtx ∗
+      P ∗
+      Ψ false ∗
+      {{{
+        mutex.(mutex_locked) mtx ∗
+        P ∗
+        Ψ false
+      }}}
+        cond #()
+      {{{ (b : bool),
+        RET #b;
+        mutex.(mutex_locked) mtx ∗
+        P ∗
+        Ψ b
+      }}}
+    }}}
+      condition_wait_until t mtx cond
+    {{{
+      RET #();
+      mutex.(mutex_locked) mtx ∗
+      P ∗
+      Ψ true
+    }}}.
+  Proof.
+    iIntros "%Φ (#Hinv & #Hmutex_inv & Hlocked & HP & HΨ & #Hcond) HΦ".
+    wp_rec. wp_pures.
+    iLöb as "HLöb".
+    wp_rec.
+    wp_smart_apply ("Hcond" with "[$]"). iIntros "%b (Hlocked & HP & HΨ)".
+    destruct b; first iSteps.
+    wp_smart_apply (condition_wait_spec _ _ _ P with "[$]"). iIntros "(Hlocked & HP)".
+    wp_smart_apply ("HLöb" with "Hlocked HP HΨ HΦ").
+  Qed.
+
+  Lemma condition_wait_while_spec Ψ t mtx cond P :
+    {{{
+      condition.(condition_inv) t ∗
+      mutex.(mutex_inv) mtx P ∗
+      mutex.(mutex_locked) mtx ∗
+      P ∗
+      Ψ true ∗
+      {{{
+        mutex.(mutex_locked) mtx ∗
+        P ∗
+        Ψ true
+      }}}
+        cond #()
+      {{{ (b : bool),
+        RET #b;
+        mutex.(mutex_locked) mtx ∗
+        P ∗
+        Ψ b
+      }}}
+    }}}
+      condition_wait_while t mtx cond
+    {{{
+      RET #();
+      mutex.(mutex_locked) mtx ∗
+      P ∗
+      Ψ false
+    }}}.
+  Proof.
+    iIntros "%Φ (#Hinv & #Hmutex_inv & Hlocked & HP & HΨ & #Hcond) HΦ".
+    wp_rec.
+    wp_smart_apply (condition_wait_until_spec (λ b, Ψ (negb b)) _ _ _ P with "[$Hlocked $HP $HΨ]"); last iSteps.
+    iFrame "#∗". clear. iIntros "%Φ !> (Hlocked & HP & HΨ) HΦ".
+    wp_smart_apply ("Hcond" with "[$]"). iIntros "%b (Hlocked & HP & HΨ)".
+    destruct b; iSteps.
+  Qed.
+End condition.
+
+#[global] Opaque condition_wait_until.
+#[global] Opaque condition_wait_while.
+
+Notation "condition .(condition_wait_until)" := (
+  condition_wait_until condition
+)(at level 5
+).
+Notation "condition .(condition_wait_while)" := (
+  condition_wait_while condition
+)(at level 5
+).
